parallel substs

pulse/src/ocaml/plugin/generated/Pulse_Syntax_Naming.ml
@@ -275,106 +275,170 @@ let (ln_st : Pulse_Syntax_Base.st_term -> Prims.bool) =
   fun t -> ln_st' t (Prims.of_int (-1))
 let (ln_c : Pulse_Syntax_Base.comp -> Prims.bool) =
   fun c -> ln_c' c (Prims.of_int (-1))
-let rec (open_term' :
+type subst_elt =
+  | DT of Prims.nat * Pulse_Syntax_Base.term 
+  | NT of Pulse_Syntax_Base.var * Pulse_Syntax_Base.term 
+  | ND of Pulse_Syntax_Base.var * Prims.nat 
+let (uu___is_DT : subst_elt -> Prims.bool) =
+  fun projectee ->
+    match projectee with | DT (_0, _1) -> true | uu___ -> false
+let (__proj__DT__item___0 : subst_elt -> Prims.nat) =
+  fun projectee -> match projectee with | DT (_0, _1) -> _0
+let (__proj__DT__item___1 : subst_elt -> Pulse_Syntax_Base.term) =
+  fun projectee -> match projectee with | DT (_0, _1) -> _1
+let (uu___is_NT : subst_elt -> Prims.bool) =
+  fun projectee ->
+    match projectee with | NT (_0, _1) -> true | uu___ -> false
+let (__proj__NT__item___0 : subst_elt -> Pulse_Syntax_Base.var) =
+  fun projectee -> match projectee with | NT (_0, _1) -> _0
+let (__proj__NT__item___1 : subst_elt -> Pulse_Syntax_Base.term) =
+  fun projectee -> match projectee with | NT (_0, _1) -> _1
+let (uu___is_ND : subst_elt -> Prims.bool) =
+  fun projectee ->
+    match projectee with | ND (_0, _1) -> true | uu___ -> false
+let (__proj__ND__item___0 : subst_elt -> Pulse_Syntax_Base.var) =
+  fun projectee -> match projectee with | ND (_0, _1) -> _0
+let (__proj__ND__item___1 : subst_elt -> Prims.nat) =
+  fun projectee -> match projectee with | ND (_0, _1) -> _1
+let (shift_subst_elt : Prims.nat -> subst_elt -> subst_elt) =
+  fun n ->
+    fun uu___ ->
+      match uu___ with
+      | DT (i, t) -> DT ((i + n), t)
+      | NT (x, t) -> NT (x, t)
+      | ND (x, i) -> ND (x, (i + n))
+type subst = subst_elt Prims.list
+let (shift_subst_n :
+  Prims.nat -> subst_elt Prims.list -> subst_elt Prims.list) =
+  fun n -> FStar_List_Tot_Base.map (shift_subst_elt n)
+let (shift_subst : subst_elt Prims.list -> subst_elt Prims.list) =
+  shift_subst_n Prims.int_one
+let (rt_subst_elt : subst_elt -> FStar_Reflection_Typing.subst_elt) =
+  fun uu___ ->
+    match uu___ with
+    | DT (i, t) ->
+        FStar_Reflection_Typing.DT (i, (Pulse_Elaborate_Pure.elab_term t))
+    | NT (x, t) ->
+        FStar_Reflection_Typing.NT (x, (Pulse_Elaborate_Pure.elab_term t))
+    | ND (x, i) -> FStar_Reflection_Typing.ND (x, i)
+let (rt_subst :
+  subst_elt Prims.list -> FStar_Reflection_Typing.subst_elt Prims.list) =
+  FStar_List_Tot_Base.map rt_subst_elt
+let rec (subst_term :
+  Pulse_Syntax_Base.term -> subst -> Pulse_Syntax_Base.term) =
+  fun t ->
+    fun ss ->
+      match t with
+      | Pulse_Syntax_Base.Tm_VProp -> t
+      | Pulse_Syntax_Base.Tm_Emp -> t
+      | Pulse_Syntax_Base.Tm_Inames -> t
+      | Pulse_Syntax_Base.Tm_EmpInames -> t
+      | Pulse_Syntax_Base.Tm_Unknown -> t
+      | Pulse_Syntax_Base.Tm_Pure p ->
+          Pulse_Syntax_Base.Tm_Pure (subst_term p ss)
+      | Pulse_Syntax_Base.Tm_Star (l, r) ->
+          Pulse_Syntax_Base.Tm_Star ((subst_term l ss), (subst_term r ss))
+      | Pulse_Syntax_Base.Tm_ExistsSL (u, b, body) ->
+          Pulse_Syntax_Base.Tm_ExistsSL
+            (u,
+              {
+                Pulse_Syntax_Base.binder_ty =
+                  (subst_term b.Pulse_Syntax_Base.binder_ty ss);
+                Pulse_Syntax_Base.binder_ppname =
+                  (b.Pulse_Syntax_Base.binder_ppname)
+              }, (subst_term body (shift_subst ss)))
+      | Pulse_Syntax_Base.Tm_ForallSL (u, b, body) ->
+          Pulse_Syntax_Base.Tm_ForallSL
+            (u,
+              {
+                Pulse_Syntax_Base.binder_ty =
+                  (subst_term b.Pulse_Syntax_Base.binder_ty ss);
+                Pulse_Syntax_Base.binder_ppname =
+                  (b.Pulse_Syntax_Base.binder_ppname)
+              }, (subst_term body (shift_subst ss)))
+      | Pulse_Syntax_Base.Tm_FStar (t1, r) ->
+          Pulse_Syntax_Base.Tm_FStar
+            ((FStar_Reflection_Typing.subst_term t1 (rt_subst ss)), r)
+let (open_term' :
   Pulse_Syntax_Base.term ->
     Pulse_Syntax_Base.term ->
       Pulse_Syntax_Base.index -> Pulse_Syntax_Base.term)
-  =
-  fun t ->
-    fun v ->
-      fun i ->
-        match t with
-        | Pulse_Syntax_Base.Tm_VProp -> t
-        | Pulse_Syntax_Base.Tm_Emp -> t
-        | Pulse_Syntax_Base.Tm_Inames -> t
-        | Pulse_Syntax_Base.Tm_EmpInames -> t
-        | Pulse_Syntax_Base.Tm_Unknown -> t
-        | Pulse_Syntax_Base.Tm_Pure p ->
-            Pulse_Syntax_Base.Tm_Pure (open_term' p v i)
-        | Pulse_Syntax_Base.Tm_Star (l, r) ->
-            Pulse_Syntax_Base.Tm_Star
-              ((open_term' l v i), (open_term' r v i))
-        | Pulse_Syntax_Base.Tm_ExistsSL (u, b, body) ->
-            Pulse_Syntax_Base.Tm_ExistsSL
-              (u,
-                {
-                  Pulse_Syntax_Base.binder_ty =
-                    (open_term' b.Pulse_Syntax_Base.binder_ty v i);
-                  Pulse_Syntax_Base.binder_ppname =
-                    (b.Pulse_Syntax_Base.binder_ppname)
-                }, (open_term' body v (i + Prims.int_one)))
-        | Pulse_Syntax_Base.Tm_ForallSL (u, b, body) ->
-            Pulse_Syntax_Base.Tm_ForallSL
-              (u,
-                {
-                  Pulse_Syntax_Base.binder_ty =
-                    (open_term' b.Pulse_Syntax_Base.binder_ty v i);
-                  Pulse_Syntax_Base.binder_ppname =
-                    (b.Pulse_Syntax_Base.binder_ppname)
-                }, (open_term' body v (i + Prims.int_one)))
-        | Pulse_Syntax_Base.Tm_FStar (t1, r) ->
-            Pulse_Syntax_Base.Tm_FStar
-              ((FStar_Reflection_Typing.subst_term t1
-                  [FStar_Reflection_Typing.DT
-                     (i, (Pulse_Elaborate_Pure.elab_term v))]), r)
+  = fun t -> fun v -> fun i -> subst_term t [DT (i, v)]
+let (subst_st_comp :
+  Pulse_Syntax_Base.st_comp -> subst -> Pulse_Syntax_Base.st_comp) =
+  fun s ->
+    fun ss ->
+      {
+        Pulse_Syntax_Base.u = (s.Pulse_Syntax_Base.u);
+        Pulse_Syntax_Base.res = (subst_term s.Pulse_Syntax_Base.res ss);
+        Pulse_Syntax_Base.pre = (subst_term s.Pulse_Syntax_Base.pre ss);
+        Pulse_Syntax_Base.post =
+          (subst_term s.Pulse_Syntax_Base.post (shift_subst ss))
+      }
 let (open_st_comp' :
   Pulse_Syntax_Base.st_comp ->
     Pulse_Syntax_Base.term ->
       Pulse_Syntax_Base.index -> Pulse_Syntax_Base.st_comp)
+  = fun s -> fun v -> fun i -> subst_st_comp s [DT (i, v)]
+let (subst_comp : Pulse_Syntax_Base.comp -> subst -> Pulse_Syntax_Base.comp)
   =
-  fun s ->
-    fun v ->
-      fun i ->
-        {
-          Pulse_Syntax_Base.u = (s.Pulse_Syntax_Base.u);
-          Pulse_Syntax_Base.res = (open_term' s.Pulse_Syntax_Base.res v i);
-          Pulse_Syntax_Base.pre = (open_term' s.Pulse_Syntax_Base.pre v i);
-          Pulse_Syntax_Base.post =
-            (open_term' s.Pulse_Syntax_Base.post v (i + Prims.int_one))
-        }
+  fun c ->
+    fun ss ->
+      match c with
+      | Pulse_Syntax_Base.C_Tot t ->
+          Pulse_Syntax_Base.C_Tot (subst_term t ss)
+      | Pulse_Syntax_Base.C_ST s ->
+          Pulse_Syntax_Base.C_ST (subst_st_comp s ss)
+      | Pulse_Syntax_Base.C_STAtomic (inames, s) ->
+          Pulse_Syntax_Base.C_STAtomic
+            ((subst_term inames ss), (subst_st_comp s ss))
+      | Pulse_Syntax_Base.C_STGhost (inames, s) ->
+          Pulse_Syntax_Base.C_STGhost
+            ((subst_term inames ss), (subst_st_comp s ss))
 let (open_comp' :
   Pulse_Syntax_Base.comp ->
     Pulse_Syntax_Base.term ->
       Pulse_Syntax_Base.index -> Pulse_Syntax_Base.comp)
+  = fun c -> fun v -> fun i -> subst_comp c [DT (i, v)]
+let (subst_term_opt :
+  Pulse_Syntax_Base.term FStar_Pervasives_Native.option ->
+    subst -> Pulse_Syntax_Base.term FStar_Pervasives_Native.option)
   =
-  fun c ->
-    fun v ->
-      fun i ->
-        match c with
-        | Pulse_Syntax_Base.C_Tot t ->
-            Pulse_Syntax_Base.C_Tot (open_term' t v i)
-        | Pulse_Syntax_Base.C_ST s ->
-            Pulse_Syntax_Base.C_ST (open_st_comp' s v i)
-        | Pulse_Syntax_Base.C_STAtomic (inames, s) ->
-            Pulse_Syntax_Base.C_STAtomic
-              ((open_term' inames v i), (open_st_comp' s v i))
-        | Pulse_Syntax_Base.C_STGhost (inames, s) ->
-            Pulse_Syntax_Base.C_STGhost
-              ((open_term' inames v i), (open_st_comp' s v i))
+  fun t ->
+    fun ss ->
+      match t with
+      | FStar_Pervasives_Native.None -> FStar_Pervasives_Native.None
+      | FStar_Pervasives_Native.Some t1 ->
+          FStar_Pervasives_Native.Some (subst_term t1 ss)
 let (open_term_opt' :
   Pulse_Syntax_Base.term FStar_Pervasives_Native.option ->
     Pulse_Syntax_Base.term ->
       Pulse_Syntax_Base.index ->
         Pulse_Syntax_Base.term FStar_Pervasives_Native.option)
+  = fun t -> fun v -> fun i -> subst_term_opt t [DT (i, v)]
+let rec (subst_term_list :
+  Pulse_Syntax_Base.term Prims.list ->
+    subst -> Pulse_Syntax_Base.term Prims.list)
   =
   fun t ->
-    fun v ->
-      fun i ->
-        match t with
-        | FStar_Pervasives_Native.None -> FStar_Pervasives_Native.None
-        | FStar_Pervasives_Native.Some t1 ->
-            FStar_Pervasives_Native.Some (open_term' t1 v i)
-let rec (open_term_list' :
+    fun ss ->
+      match t with
+      | [] -> []
+      | hd::tl -> (subst_term hd ss) :: (subst_term_list tl ss)
+let (open_term_list' :
   Pulse_Syntax_Base.term Prims.list ->
     Pulse_Syntax_Base.term ->
       Pulse_Syntax_Base.index -> Pulse_Syntax_Base.term Prims.list)
-  =
-  fun t ->
-    fun v ->
-      fun i ->
-        match t with
-        | [] -> []
-        | hd::tl -> (open_term' hd v i) :: (open_term_list' tl v i)
+  = fun t -> fun v -> fun i -> subst_term_list t [DT (i, v)]
+let (subst_binder :
+  Pulse_Syntax_Base.binder -> subst -> Pulse_Syntax_Base.binder) =
+  fun b ->
+    fun ss ->
+      {
+        Pulse_Syntax_Base.binder_ty =
+          (subst_term b.Pulse_Syntax_Base.binder_ty ss);
+        Pulse_Syntax_Base.binder_ppname = (b.Pulse_Syntax_Base.binder_ppname)
+      }
 let (open_binder :
   Pulse_Syntax_Base.binder ->
     Pulse_Syntax_Base.term ->
@@ -389,190 +453,188 @@ let (open_binder :
           Pulse_Syntax_Base.binder_ppname =
             (b.Pulse_Syntax_Base.binder_ppname)
         }
-let rec (open_st_term' :
+let rec (subst_st_term :
+  Pulse_Syntax_Base.st_term -> subst -> Pulse_Syntax_Base.st_term) =
+  fun t ->
+    fun ss ->
+      let t' =
+        match t.Pulse_Syntax_Base.term1 with
+        | Pulse_Syntax_Base.Tm_Return
+            { Pulse_Syntax_Base.ctag = ctag;
+              Pulse_Syntax_Base.insert_eq = insert_eq;
+              Pulse_Syntax_Base.term = term;_}
+            ->
+            Pulse_Syntax_Base.Tm_Return
+              {
+                Pulse_Syntax_Base.ctag = ctag;
+                Pulse_Syntax_Base.insert_eq = insert_eq;
+                Pulse_Syntax_Base.term = (subst_term term ss)
+              }
+        | Pulse_Syntax_Base.Tm_Abs
+            { Pulse_Syntax_Base.b = b; Pulse_Syntax_Base.q = q;
+              Pulse_Syntax_Base.pre1 = pre; Pulse_Syntax_Base.body = body;
+              Pulse_Syntax_Base.ret_ty = ret_ty;
+              Pulse_Syntax_Base.post1 = post;_}
+            ->
+            Pulse_Syntax_Base.Tm_Abs
+              {
+                Pulse_Syntax_Base.b = (subst_binder b ss);
+                Pulse_Syntax_Base.q = q;
+                Pulse_Syntax_Base.pre1 =
+                  (subst_term_opt pre (shift_subst ss));
+                Pulse_Syntax_Base.body =
+                  (subst_st_term body (shift_subst ss));
+                Pulse_Syntax_Base.ret_ty =
+                  (subst_term_opt ret_ty (shift_subst ss));
+                Pulse_Syntax_Base.post1 =
+                  (subst_term_opt post (shift_subst_n (Prims.of_int (2)) ss))
+              }
+        | Pulse_Syntax_Base.Tm_STApp
+            { Pulse_Syntax_Base.head = head;
+              Pulse_Syntax_Base.arg_qual = arg_qual;
+              Pulse_Syntax_Base.arg = arg;_}
+            ->
+            Pulse_Syntax_Base.Tm_STApp
+              {
+                Pulse_Syntax_Base.head = (subst_term head ss);
+                Pulse_Syntax_Base.arg_qual = arg_qual;
+                Pulse_Syntax_Base.arg = (subst_term arg ss)
+              }
+        | Pulse_Syntax_Base.Tm_Bind
+            { Pulse_Syntax_Base.binder = binder;
+              Pulse_Syntax_Base.head1 = head;
+              Pulse_Syntax_Base.body1 = body;_}
+            ->
+            Pulse_Syntax_Base.Tm_Bind
+              {
+                Pulse_Syntax_Base.binder = (subst_binder binder ss);
+                Pulse_Syntax_Base.head1 = (subst_st_term head ss);
+                Pulse_Syntax_Base.body1 =
+                  (subst_st_term body (shift_subst ss))
+              }
+        | Pulse_Syntax_Base.Tm_TotBind
+            { Pulse_Syntax_Base.head2 = head;
+              Pulse_Syntax_Base.body2 = body;_}
+            ->
+            Pulse_Syntax_Base.Tm_TotBind
+              {
+                Pulse_Syntax_Base.head2 = (subst_term head ss);
+                Pulse_Syntax_Base.body2 =
+                  (subst_st_term body (shift_subst ss))
+              }
+        | Pulse_Syntax_Base.Tm_If
+            { Pulse_Syntax_Base.b1 = b; Pulse_Syntax_Base.then_ = then_;
+              Pulse_Syntax_Base.else_ = else_;
+              Pulse_Syntax_Base.post2 = post;_}
+            ->
+            Pulse_Syntax_Base.Tm_If
+              {
+                Pulse_Syntax_Base.b1 = (subst_term b ss);
+                Pulse_Syntax_Base.then_ = (subst_st_term then_ ss);
+                Pulse_Syntax_Base.else_ = (subst_st_term else_ ss);
+                Pulse_Syntax_Base.post2 =
+                  (subst_term_opt post (shift_subst ss))
+              }
+        | Pulse_Syntax_Base.Tm_IntroPure
+            { Pulse_Syntax_Base.p = p;
+              Pulse_Syntax_Base.should_check = should_check;_}
+            ->
+            Pulse_Syntax_Base.Tm_IntroPure
+              {
+                Pulse_Syntax_Base.p = (subst_term p ss);
+                Pulse_Syntax_Base.should_check = should_check
+              }
+        | Pulse_Syntax_Base.Tm_ElimExists { Pulse_Syntax_Base.p1 = p;_} ->
+            Pulse_Syntax_Base.Tm_ElimExists
+              { Pulse_Syntax_Base.p1 = (subst_term p ss) }
+        | Pulse_Syntax_Base.Tm_IntroExists
+            { Pulse_Syntax_Base.erased = erased; Pulse_Syntax_Base.p2 = p;
+              Pulse_Syntax_Base.witnesses = witnesses;
+              Pulse_Syntax_Base.should_check1 = should_check;_}
+            ->
+            Pulse_Syntax_Base.Tm_IntroExists
+              {
+                Pulse_Syntax_Base.erased = erased;
+                Pulse_Syntax_Base.p2 = (subst_term p ss);
+                Pulse_Syntax_Base.witnesses = (subst_term_list witnesses ss);
+                Pulse_Syntax_Base.should_check1 = should_check
+              }
+        | Pulse_Syntax_Base.Tm_While
+            { Pulse_Syntax_Base.invariant = invariant;
+              Pulse_Syntax_Base.condition = condition;
+              Pulse_Syntax_Base.condition_var = condition_var;
+              Pulse_Syntax_Base.body3 = body;_}
+            ->
+            Pulse_Syntax_Base.Tm_While
+              {
+                Pulse_Syntax_Base.invariant =
+                  (subst_term invariant (shift_subst ss));
+                Pulse_Syntax_Base.condition = (subst_st_term condition ss);
+                Pulse_Syntax_Base.condition_var = condition_var;
+                Pulse_Syntax_Base.body3 = (subst_st_term body ss)
+              }
+        | Pulse_Syntax_Base.Tm_Par
+            { Pulse_Syntax_Base.pre11 = pre1;
+              Pulse_Syntax_Base.body11 = body1;
+              Pulse_Syntax_Base.post11 = post1;
+              Pulse_Syntax_Base.pre2 = pre2;
+              Pulse_Syntax_Base.body21 = body2;
+              Pulse_Syntax_Base.post21 = post2;_}
+            ->
+            Pulse_Syntax_Base.Tm_Par
+              {
+                Pulse_Syntax_Base.pre11 = (subst_term pre1 ss);
+                Pulse_Syntax_Base.body11 = (subst_st_term body1 ss);
+                Pulse_Syntax_Base.post11 =
+                  (subst_term post1 (shift_subst ss));
+                Pulse_Syntax_Base.pre2 = (subst_term pre2 ss);
+                Pulse_Syntax_Base.body21 = (subst_st_term body2 ss);
+                Pulse_Syntax_Base.post21 =
+                  (subst_term post2 (shift_subst ss))
+              }
+        | Pulse_Syntax_Base.Tm_WithLocal
+            { Pulse_Syntax_Base.binder1 = binder;
+              Pulse_Syntax_Base.initializer1 = initializer1;
+              Pulse_Syntax_Base.body4 = body;_}
+            ->
+            Pulse_Syntax_Base.Tm_WithLocal
+              {
+                Pulse_Syntax_Base.binder1 = (subst_binder binder ss);
+                Pulse_Syntax_Base.initializer1 = (subst_term initializer1 ss);
+                Pulse_Syntax_Base.body4 =
+                  (subst_st_term body (shift_subst ss))
+              }
+        | Pulse_Syntax_Base.Tm_Rewrite
+            { Pulse_Syntax_Base.t1 = t1; Pulse_Syntax_Base.t2 = t2;_} ->
+            Pulse_Syntax_Base.Tm_Rewrite
+              {
+                Pulse_Syntax_Base.t1 = (subst_term t1 ss);
+                Pulse_Syntax_Base.t2 = (subst_term t2 ss)
+              }
+        | Pulse_Syntax_Base.Tm_Admit
+            { Pulse_Syntax_Base.ctag1 = ctag; Pulse_Syntax_Base.u1 = u;
+              Pulse_Syntax_Base.typ = typ; Pulse_Syntax_Base.post3 = post;_}
+            ->
+            Pulse_Syntax_Base.Tm_Admit
+              {
+                Pulse_Syntax_Base.ctag1 = ctag;
+                Pulse_Syntax_Base.u1 = u;
+                Pulse_Syntax_Base.typ = (subst_term typ ss);
+                Pulse_Syntax_Base.post3 =
+                  (subst_term_opt post (shift_subst ss))
+              }
+        | Pulse_Syntax_Base.Tm_Protect { Pulse_Syntax_Base.t = t1;_} ->
+            Pulse_Syntax_Base.Tm_Protect
+              { Pulse_Syntax_Base.t = (subst_st_term t1 ss) } in
+      {
+        Pulse_Syntax_Base.term1 = t';
+        Pulse_Syntax_Base.range1 = (t.Pulse_Syntax_Base.range1)
+      }
+let (open_st_term' :
   Pulse_Syntax_Base.st_term ->
     Pulse_Syntax_Base.term ->
       Pulse_Syntax_Base.index -> Pulse_Syntax_Base.st_term)
-  =
-  fun t ->
-    fun v ->
-      fun i ->
-        let t' =
-          match t.Pulse_Syntax_Base.term1 with
-          | Pulse_Syntax_Base.Tm_Return
-              { Pulse_Syntax_Base.ctag = ctag;
-                Pulse_Syntax_Base.insert_eq = insert_eq;
-                Pulse_Syntax_Base.term = term;_}
-              ->
-              Pulse_Syntax_Base.Tm_Return
-                {
-                  Pulse_Syntax_Base.ctag = ctag;
-                  Pulse_Syntax_Base.insert_eq = insert_eq;
-                  Pulse_Syntax_Base.term = (open_term' term v i)
-                }
-          | Pulse_Syntax_Base.Tm_Abs
-              { Pulse_Syntax_Base.b = b; Pulse_Syntax_Base.q = q;
-                Pulse_Syntax_Base.pre1 = pre; Pulse_Syntax_Base.body = body;
-                Pulse_Syntax_Base.ret_ty = ret_ty;
-                Pulse_Syntax_Base.post1 = post;_}
-              ->
-              Pulse_Syntax_Base.Tm_Abs
-                {
-                  Pulse_Syntax_Base.b = (open_binder b v i);
-                  Pulse_Syntax_Base.q = q;
-                  Pulse_Syntax_Base.pre1 =
-                    (open_term_opt' pre v (i + Prims.int_one));
-                  Pulse_Syntax_Base.body =
-                    (open_st_term' body v (i + Prims.int_one));
-                  Pulse_Syntax_Base.ret_ty =
-                    (open_term_opt' ret_ty v (i + Prims.int_one));
-                  Pulse_Syntax_Base.post1 =
-                    (open_term_opt' post v (i + (Prims.of_int (2))))
-                }
-          | Pulse_Syntax_Base.Tm_STApp
-              { Pulse_Syntax_Base.head = head;
-                Pulse_Syntax_Base.arg_qual = arg_qual;
-                Pulse_Syntax_Base.arg = arg;_}
-              ->
-              Pulse_Syntax_Base.Tm_STApp
-                {
-                  Pulse_Syntax_Base.head = (open_term' head v i);
-                  Pulse_Syntax_Base.arg_qual = arg_qual;
-                  Pulse_Syntax_Base.arg = (open_term' arg v i)
-                }
-          | Pulse_Syntax_Base.Tm_Bind
-              { Pulse_Syntax_Base.binder = binder;
-                Pulse_Syntax_Base.head1 = head;
-                Pulse_Syntax_Base.body1 = body;_}
-              ->
-              Pulse_Syntax_Base.Tm_Bind
-                {
-                  Pulse_Syntax_Base.binder = (open_binder binder v i);
-                  Pulse_Syntax_Base.head1 = (open_st_term' head v i);
-                  Pulse_Syntax_Base.body1 =
-                    (open_st_term' body v (i + Prims.int_one))
-                }
-          | Pulse_Syntax_Base.Tm_TotBind
-              { Pulse_Syntax_Base.head2 = head;
-                Pulse_Syntax_Base.body2 = body;_}
-              ->
-              Pulse_Syntax_Base.Tm_TotBind
-                {
-                  Pulse_Syntax_Base.head2 = (open_term' head v i);
-                  Pulse_Syntax_Base.body2 =
-                    (open_st_term' body v (i + Prims.int_one))
-                }
-          | Pulse_Syntax_Base.Tm_If
-              { Pulse_Syntax_Base.b1 = b; Pulse_Syntax_Base.then_ = then_;
-                Pulse_Syntax_Base.else_ = else_;
-                Pulse_Syntax_Base.post2 = post;_}
-              ->
-              Pulse_Syntax_Base.Tm_If
-                {
-                  Pulse_Syntax_Base.b1 = (open_term' b v i);
-                  Pulse_Syntax_Base.then_ = (open_st_term' then_ v i);
-                  Pulse_Syntax_Base.else_ = (open_st_term' else_ v i);
-                  Pulse_Syntax_Base.post2 =
-                    (open_term_opt' post v (i + Prims.int_one))
-                }
-          | Pulse_Syntax_Base.Tm_IntroPure
-              { Pulse_Syntax_Base.p = p;
-                Pulse_Syntax_Base.should_check = should_check;_}
-              ->
-              Pulse_Syntax_Base.Tm_IntroPure
-                {
-                  Pulse_Syntax_Base.p = (open_term' p v i);
-                  Pulse_Syntax_Base.should_check = should_check
-                }
-          | Pulse_Syntax_Base.Tm_ElimExists { Pulse_Syntax_Base.p1 = p;_} ->
-              Pulse_Syntax_Base.Tm_ElimExists
-                { Pulse_Syntax_Base.p1 = (open_term' p v i) }
-          | Pulse_Syntax_Base.Tm_IntroExists
-              { Pulse_Syntax_Base.erased = erased; Pulse_Syntax_Base.p2 = p;
-                Pulse_Syntax_Base.witnesses = witnesses;
-                Pulse_Syntax_Base.should_check1 = should_check;_}
-              ->
-              Pulse_Syntax_Base.Tm_IntroExists
-                {
-                  Pulse_Syntax_Base.erased = erased;
-                  Pulse_Syntax_Base.p2 = (open_term' p v i);
-                  Pulse_Syntax_Base.witnesses =
-                    (open_term_list' witnesses v i);
-                  Pulse_Syntax_Base.should_check1 = should_check
-                }
-          | Pulse_Syntax_Base.Tm_While
-              { Pulse_Syntax_Base.invariant = invariant;
-                Pulse_Syntax_Base.condition = condition;
-                Pulse_Syntax_Base.condition_var = condition_var;
-                Pulse_Syntax_Base.body3 = body;_}
-              ->
-              Pulse_Syntax_Base.Tm_While
-                {
-                  Pulse_Syntax_Base.invariant =
-                    (open_term' invariant v (i + Prims.int_one));
-                  Pulse_Syntax_Base.condition = (open_st_term' condition v i);
-                  Pulse_Syntax_Base.condition_var = condition_var;
-                  Pulse_Syntax_Base.body3 = (open_st_term' body v i)
-                }
-          | Pulse_Syntax_Base.Tm_Par
-              { Pulse_Syntax_Base.pre11 = pre1;
-                Pulse_Syntax_Base.body11 = body1;
-                Pulse_Syntax_Base.post11 = post1;
-                Pulse_Syntax_Base.pre2 = pre2;
-                Pulse_Syntax_Base.body21 = body2;
-                Pulse_Syntax_Base.post21 = post2;_}
-              ->
-              Pulse_Syntax_Base.Tm_Par
-                {
-                  Pulse_Syntax_Base.pre11 = (open_term' pre1 v i);
-                  Pulse_Syntax_Base.body11 = (open_st_term' body1 v i);
-                  Pulse_Syntax_Base.post11 =
-                    (open_term' post1 v (i + Prims.int_one));
-                  Pulse_Syntax_Base.pre2 = (open_term' pre2 v i);
-                  Pulse_Syntax_Base.body21 = (open_st_term' body2 v i);
-                  Pulse_Syntax_Base.post21 =
-                    (open_term' post2 v (i + Prims.int_one))
-                }
-          | Pulse_Syntax_Base.Tm_WithLocal
-              { Pulse_Syntax_Base.binder1 = binder;
-                Pulse_Syntax_Base.initializer1 = initializer1;
-                Pulse_Syntax_Base.body4 = body;_}
-              ->
-              Pulse_Syntax_Base.Tm_WithLocal
-                {
-                  Pulse_Syntax_Base.binder1 = (open_binder binder v i);
-                  Pulse_Syntax_Base.initializer1 =
-                    (open_term' initializer1 v i);
-                  Pulse_Syntax_Base.body4 =
-                    (open_st_term' body v (i + Prims.int_one))
-                }
-          | Pulse_Syntax_Base.Tm_Rewrite
-              { Pulse_Syntax_Base.t1 = t1; Pulse_Syntax_Base.t2 = t2;_} ->
-              Pulse_Syntax_Base.Tm_Rewrite
-                {
-                  Pulse_Syntax_Base.t1 = (open_term' t1 v i);
-                  Pulse_Syntax_Base.t2 = (open_term' t2 v i)
-                }
-          | Pulse_Syntax_Base.Tm_Admit
-              { Pulse_Syntax_Base.ctag1 = ctag; Pulse_Syntax_Base.u1 = u;
-                Pulse_Syntax_Base.typ = typ;
-                Pulse_Syntax_Base.post3 = post;_}
-              ->
-              Pulse_Syntax_Base.Tm_Admit
-                {
-                  Pulse_Syntax_Base.ctag1 = ctag;
-                  Pulse_Syntax_Base.u1 = u;
-                  Pulse_Syntax_Base.typ = (open_term' typ v i);
-                  Pulse_Syntax_Base.post3 =
-                    (open_term_opt' post v (i + Prims.int_one))
-                }
-          | Pulse_Syntax_Base.Tm_Protect { Pulse_Syntax_Base.t = t1;_} ->
-              Pulse_Syntax_Base.Tm_Protect
-                { Pulse_Syntax_Base.t = (open_st_term' t1 v i) } in
-        {
-          Pulse_Syntax_Base.term1 = t';
-          Pulse_Syntax_Base.range1 = (t.Pulse_Syntax_Base.range1)
-        }
+  = fun t -> fun v -> fun i -> subst_st_term t [DT (i, v)]
 let (open_term_nv :
   Pulse_Syntax_Base.term -> Pulse_Syntax_Base.nvar -> Pulse_Syntax_Base.term)
   =
@@ -588,304 +650,41 @@ let (open_st_term_nv :
 let (open_comp_with :
   Pulse_Syntax_Base.comp -> Pulse_Syntax_Base.term -> Pulse_Syntax_Base.comp)
   = fun c -> fun x -> open_comp' c x Prims.int_zero
-let rec (close_term' :
+let (close_term' :
   Pulse_Syntax_Base.term ->
     Pulse_Syntax_Base.var ->
       Pulse_Syntax_Base.index -> Pulse_Syntax_Base.term)
-  =
-  fun t ->
-    fun v ->
-      fun i ->
-        match t with
-        | Pulse_Syntax_Base.Tm_VProp -> t
-        | Pulse_Syntax_Base.Tm_Emp -> t
-        | Pulse_Syntax_Base.Tm_Inames -> t
-        | Pulse_Syntax_Base.Tm_EmpInames -> t
-        | Pulse_Syntax_Base.Tm_Unknown -> t
-        | Pulse_Syntax_Base.Tm_Pure p ->
-            Pulse_Syntax_Base.Tm_Pure (close_term' p v i)
-        | Pulse_Syntax_Base.Tm_Star (l, r) ->
-            Pulse_Syntax_Base.Tm_Star
-              ((close_term' l v i), (close_term' r v i))
-        | Pulse_Syntax_Base.Tm_ExistsSL (u, b, body) ->
-            Pulse_Syntax_Base.Tm_ExistsSL
-              (u,
-                {
-                  Pulse_Syntax_Base.binder_ty =
-                    (close_term' b.Pulse_Syntax_Base.binder_ty v i);
-                  Pulse_Syntax_Base.binder_ppname =
-                    (b.Pulse_Syntax_Base.binder_ppname)
-                }, (close_term' body v (i + Prims.int_one)))
-        | Pulse_Syntax_Base.Tm_ForallSL (u, b, body) ->
-            Pulse_Syntax_Base.Tm_ForallSL
-              (u,
-                {
-                  Pulse_Syntax_Base.binder_ty =
-                    (close_term' b.Pulse_Syntax_Base.binder_ty v i);
-                  Pulse_Syntax_Base.binder_ppname =
-                    (b.Pulse_Syntax_Base.binder_ppname)
-                }, (close_term' body v (i + Prims.int_one)))
-        | Pulse_Syntax_Base.Tm_FStar (t1, r) ->
-            Pulse_Syntax_Base.Tm_FStar
-              ((FStar_Reflection_Typing.subst_term t1
-                  [FStar_Reflection_Typing.ND (v, i)]), r)
+  = fun t -> fun v -> fun i -> subst_term t [ND (v, i)]
 let (close_st_comp' :
   Pulse_Syntax_Base.st_comp ->
     Pulse_Syntax_Base.var ->
       Pulse_Syntax_Base.index -> Pulse_Syntax_Base.st_comp)
-  =
-  fun s ->
-    fun v ->
-      fun i ->
-        {
-          Pulse_Syntax_Base.u = (s.Pulse_Syntax_Base.u);
-          Pulse_Syntax_Base.res = (close_term' s.Pulse_Syntax_Base.res v i);
-          Pulse_Syntax_Base.pre = (close_term' s.Pulse_Syntax_Base.pre v i);
-          Pulse_Syntax_Base.post =
-            (close_term' s.Pulse_Syntax_Base.post v (i + Prims.int_one))
-        }
+  = fun s -> fun v -> fun i -> subst_st_comp s [ND (v, i)]
 let (close_comp' :
   Pulse_Syntax_Base.comp ->
     Pulse_Syntax_Base.var ->
       Pulse_Syntax_Base.index -> Pulse_Syntax_Base.comp)
-  =
-  fun c ->
-    fun v ->
-      fun i ->
-        match c with
-        | Pulse_Syntax_Base.C_Tot t ->
-            Pulse_Syntax_Base.C_Tot (close_term' t v i)
-        | Pulse_Syntax_Base.C_ST s ->
-            Pulse_Syntax_Base.C_ST (close_st_comp' s v i)
-        | Pulse_Syntax_Base.C_STAtomic (inames, s) ->
-            Pulse_Syntax_Base.C_STAtomic
-              ((close_term' inames v i), (close_st_comp' s v i))
-        | Pulse_Syntax_Base.C_STGhost (inames, s) ->
-            Pulse_Syntax_Base.C_STGhost
-              ((close_term' inames v i), (close_st_comp' s v i))
+  = fun c -> fun v -> fun i -> subst_comp c [ND (v, i)]
 let (close_term_opt' :
   Pulse_Syntax_Base.term FStar_Pervasives_Native.option ->
     Pulse_Syntax_Base.var ->
       Pulse_Syntax_Base.index ->
         Pulse_Syntax_Base.term FStar_Pervasives_Native.option)
-  =
-  fun t ->
-    fun v ->
-      fun i ->
-        match t with
-        | FStar_Pervasives_Native.None -> FStar_Pervasives_Native.None
-        | FStar_Pervasives_Native.Some t1 ->
-            FStar_Pervasives_Native.Some (close_term' t1 v i)
-let rec (close_term_list' :
+  = fun t -> fun v -> fun i -> subst_term_opt t [ND (v, i)]
+let (close_term_list' :
   Pulse_Syntax_Base.term Prims.list ->
     Pulse_Syntax_Base.var ->
       Pulse_Syntax_Base.index -> Pulse_Syntax_Base.term Prims.list)
-  =
-  fun t ->
-    fun v ->
-      fun i ->
-        match t with
-        | [] -> []
-        | hd::tl -> (close_term' hd v i) :: (close_term_list' tl v i)
+  = fun t -> fun v -> fun i -> subst_term_list t [ND (v, i)]
 let (close_binder :
   Pulse_Syntax_Base.binder ->
-    Pulse_Syntax_Base.var ->
-      Pulse_Syntax_Base.index -> Pulse_Syntax_Base.binder)
-  =
-  fun b ->
-    fun v ->
-      fun i ->
-        {
-          Pulse_Syntax_Base.binder_ty =
-            (close_term' b.Pulse_Syntax_Base.binder_ty v i);
-          Pulse_Syntax_Base.binder_ppname =
-            (b.Pulse_Syntax_Base.binder_ppname)
-        }
-let rec (close_st_term' :
+    Pulse_Syntax_Base.var -> Prims.nat -> Pulse_Syntax_Base.binder)
+  = fun b -> fun v -> fun i -> subst_binder b [ND (v, i)]
+let (close_st_term' :
   Pulse_Syntax_Base.st_term ->
     Pulse_Syntax_Base.var ->
       Pulse_Syntax_Base.index -> Pulse_Syntax_Base.st_term)
-  =
-  fun t ->
-    fun v ->
-      fun i ->
-        let t' =
-          match t.Pulse_Syntax_Base.term1 with
-          | Pulse_Syntax_Base.Tm_Return
-              { Pulse_Syntax_Base.ctag = ctag;
-                Pulse_Syntax_Base.insert_eq = insert_eq;
-                Pulse_Syntax_Base.term = term;_}
-              ->
-              Pulse_Syntax_Base.Tm_Return
-                {
-                  Pulse_Syntax_Base.ctag = ctag;
-                  Pulse_Syntax_Base.insert_eq = insert_eq;
-                  Pulse_Syntax_Base.term = (close_term' term v i)
-                }
-          | Pulse_Syntax_Base.Tm_Abs
-              { Pulse_Syntax_Base.b = b; Pulse_Syntax_Base.q = q;
-                Pulse_Syntax_Base.pre1 = pre; Pulse_Syntax_Base.body = body;
-                Pulse_Syntax_Base.ret_ty = ret_ty;
-                Pulse_Syntax_Base.post1 = post;_}
-              ->
-              Pulse_Syntax_Base.Tm_Abs
-                {
-                  Pulse_Syntax_Base.b = (close_binder b v i);
-                  Pulse_Syntax_Base.q = q;
-                  Pulse_Syntax_Base.pre1 =
-                    (close_term_opt' pre v (i + Prims.int_one));
-                  Pulse_Syntax_Base.body =
-                    (close_st_term' body v (i + Prims.int_one));
-                  Pulse_Syntax_Base.ret_ty =
-                    (close_term_opt' ret_ty v (i + Prims.int_one));
-                  Pulse_Syntax_Base.post1 =
-                    (close_term_opt' post v (i + (Prims.of_int (2))))
-                }
-          | Pulse_Syntax_Base.Tm_STApp
-              { Pulse_Syntax_Base.head = head;
-                Pulse_Syntax_Base.arg_qual = arg_qual;
-                Pulse_Syntax_Base.arg = arg;_}
-              ->
-              Pulse_Syntax_Base.Tm_STApp
-                {
-                  Pulse_Syntax_Base.head = (close_term' head v i);
-                  Pulse_Syntax_Base.arg_qual = arg_qual;
-                  Pulse_Syntax_Base.arg = (close_term' arg v i)
-                }
-          | Pulse_Syntax_Base.Tm_Bind
-              { Pulse_Syntax_Base.binder = binder;
-                Pulse_Syntax_Base.head1 = head;
-                Pulse_Syntax_Base.body1 = body;_}
-              ->
-              Pulse_Syntax_Base.Tm_Bind
-                {
-                  Pulse_Syntax_Base.binder = (close_binder binder v i);
-                  Pulse_Syntax_Base.head1 = (close_st_term' head v i);
-                  Pulse_Syntax_Base.body1 =
-                    (close_st_term' body v (i + Prims.int_one))
-                }
-          | Pulse_Syntax_Base.Tm_TotBind
-              { Pulse_Syntax_Base.head2 = head;
-                Pulse_Syntax_Base.body2 = body;_}
-              ->
-              Pulse_Syntax_Base.Tm_TotBind
-                {
-                  Pulse_Syntax_Base.head2 = (close_term' head v i);
-                  Pulse_Syntax_Base.body2 =
-                    (close_st_term' body v (i + Prims.int_one))
-                }
-          | Pulse_Syntax_Base.Tm_If
-              { Pulse_Syntax_Base.b1 = b; Pulse_Syntax_Base.then_ = then_;
-                Pulse_Syntax_Base.else_ = else_;
-                Pulse_Syntax_Base.post2 = post;_}
-              ->
-              Pulse_Syntax_Base.Tm_If
-                {
-                  Pulse_Syntax_Base.b1 = (close_term' b v i);
-                  Pulse_Syntax_Base.then_ = (close_st_term' then_ v i);
-                  Pulse_Syntax_Base.else_ = (close_st_term' else_ v i);
-                  Pulse_Syntax_Base.post2 =
-                    (close_term_opt' post v (i + Prims.int_one))
-                }
-          | Pulse_Syntax_Base.Tm_IntroPure
-              { Pulse_Syntax_Base.p = p;
-                Pulse_Syntax_Base.should_check = should_check;_}
-              ->
-              Pulse_Syntax_Base.Tm_IntroPure
-                {
-                  Pulse_Syntax_Base.p = (close_term' p v i);
-                  Pulse_Syntax_Base.should_check = should_check
-                }
-          | Pulse_Syntax_Base.Tm_ElimExists { Pulse_Syntax_Base.p1 = p;_} ->
-              Pulse_Syntax_Base.Tm_ElimExists
-                { Pulse_Syntax_Base.p1 = (close_term' p v i) }
-          | Pulse_Syntax_Base.Tm_IntroExists
-              { Pulse_Syntax_Base.erased = erased; Pulse_Syntax_Base.p2 = p;
-                Pulse_Syntax_Base.witnesses = witnesses;
-                Pulse_Syntax_Base.should_check1 = should_check;_}
-              ->
-              Pulse_Syntax_Base.Tm_IntroExists
-                {
-                  Pulse_Syntax_Base.erased = erased;
-                  Pulse_Syntax_Base.p2 = (close_term' p v i);
-                  Pulse_Syntax_Base.witnesses =
-                    (close_term_list' witnesses v i);
-                  Pulse_Syntax_Base.should_check1 = should_check
-                }
-          | Pulse_Syntax_Base.Tm_While
-              { Pulse_Syntax_Base.invariant = invariant;
-                Pulse_Syntax_Base.condition = condition;
-                Pulse_Syntax_Base.condition_var = condition_var;
-                Pulse_Syntax_Base.body3 = body;_}
-              ->
-              Pulse_Syntax_Base.Tm_While
-                {
-                  Pulse_Syntax_Base.invariant =
-                    (close_term' invariant v (i + Prims.int_one));
-                  Pulse_Syntax_Base.condition =
-                    (close_st_term' condition v i);
-                  Pulse_Syntax_Base.condition_var = condition_var;
-                  Pulse_Syntax_Base.body3 = (close_st_term' body v i)
-                }
-          | Pulse_Syntax_Base.Tm_Par
-              { Pulse_Syntax_Base.pre11 = pre1;
-                Pulse_Syntax_Base.body11 = body1;
-                Pulse_Syntax_Base.post11 = post1;
-                Pulse_Syntax_Base.pre2 = pre2;
-                Pulse_Syntax_Base.body21 = body2;
-                Pulse_Syntax_Base.post21 = post2;_}
-              ->
-              Pulse_Syntax_Base.Tm_Par
-                {
-                  Pulse_Syntax_Base.pre11 = (close_term' pre1 v i);
-                  Pulse_Syntax_Base.body11 = (close_st_term' body1 v i);
-                  Pulse_Syntax_Base.post11 =
-                    (close_term' post1 v (i + Prims.int_one));
-                  Pulse_Syntax_Base.pre2 = (close_term' pre2 v i);
-                  Pulse_Syntax_Base.body21 = (close_st_term' body2 v i);
-                  Pulse_Syntax_Base.post21 =
-                    (close_term' post2 v (i + Prims.int_one))
-                }
-          | Pulse_Syntax_Base.Tm_WithLocal
-              { Pulse_Syntax_Base.binder1 = binder;
-                Pulse_Syntax_Base.initializer1 = initializer1;
-                Pulse_Syntax_Base.body4 = body;_}
-              ->
-              Pulse_Syntax_Base.Tm_WithLocal
-                {
-                  Pulse_Syntax_Base.binder1 = (close_binder binder v i);
-                  Pulse_Syntax_Base.initializer1 =
-                    (close_term' initializer1 v i);
-                  Pulse_Syntax_Base.body4 =
-                    (close_st_term' body v (i + Prims.int_one))
-                }
-          | Pulse_Syntax_Base.Tm_Rewrite
-              { Pulse_Syntax_Base.t1 = t1; Pulse_Syntax_Base.t2 = t2;_} ->
-              Pulse_Syntax_Base.Tm_Rewrite
-                {
-                  Pulse_Syntax_Base.t1 = (close_term' t1 v i);
-                  Pulse_Syntax_Base.t2 = (close_term' t2 v i)
-                }
-          | Pulse_Syntax_Base.Tm_Admit
-              { Pulse_Syntax_Base.ctag1 = ctag; Pulse_Syntax_Base.u1 = u;
-                Pulse_Syntax_Base.typ = typ;
-                Pulse_Syntax_Base.post3 = post;_}
-              ->
-              Pulse_Syntax_Base.Tm_Admit
-                {
-                  Pulse_Syntax_Base.ctag1 = ctag;
-                  Pulse_Syntax_Base.u1 = u;
-                  Pulse_Syntax_Base.typ = (close_term' typ v i);
-                  Pulse_Syntax_Base.post3 =
-                    (close_term_opt' post v (i + Prims.int_one))
-                }
-          | Pulse_Syntax_Base.Tm_Protect { Pulse_Syntax_Base.t = t1;_} ->
-              Pulse_Syntax_Base.Tm_Protect
-                { Pulse_Syntax_Base.t = (close_st_term' t1 v i) } in
-        {
-          Pulse_Syntax_Base.term1 = t';
-          Pulse_Syntax_Base.range1 = (t.Pulse_Syntax_Base.range1)
-        }
+  = fun t -> fun v -> fun i -> subst_st_term t [ND (v, i)]
 let (close_term :
   Pulse_Syntax_Base.term -> Pulse_Syntax_Base.var -> Pulse_Syntax_Base.term)
   = fun t -> fun v -> close_term' t v Prims.int_zero
